theories/Substitution/Introductions/Sigma.v
@@ -522,9 +522,9 @@ Section PairRed.
         Unshelve. tea.
     + eapply convtm_eta_sig; tea.
       * now eapply ty_pair.
-      * constructor; unshelve eapply escapeEq, reflLRTyEq; [|tea].
+      * constructor; tea; (unshelve eapply escapeEq, reflLRTyEq; [|tea]).
       * now eapply ty_pair.
-      * constructor; unshelve eapply escapeEq, reflLRTyEq; [|tea].
+      * constructor; tea; (unshelve eapply escapeEq, reflLRTyEq; [|tea]).
       * enough [Γ |- tFst (tPair A B a b) ≅ a : A].
         1: transitivity a; tea; now symmetry.
         eapply convtm_exp.
@@ -553,13 +553,64 @@ Section PairRed.
       Unshelve. all: tea.
   Qed.
 
-  Lemma isLRPair_isWfPair {Γ A B l p} (wfΓ : [|- Γ]) (ΣA : [Γ ||-Σ<l> tSig A B]) (Rp : [Γ ||-Σ p : _ | normRedΣ0 ΣA]) :
+  Lemma isLRPair_isWfPair {Γ A B l p} (wfΓ : [|- Γ]) (ΣA : [Γ ||-Σ<l> tSig A B])
+  (RA : [Γ ||-<l> A])
+  (Rp : [Γ ||-Σ p : _ | normRedΣ0 ΣA]) :
     isWfPair Γ A B (SigRedTm.nf Rp).
   Proof.
   destruct Rp; simpl; intros.
-  destruct ispair as [A' B' a b HA|]; constructor; tea.
-  rewrite <- (wk_id_ren_on Γ A), <- (wk_id_ren_on Γ A').
-  eapply escapeEq; now unshelve apply HA.
+  destruct ispair as [A' B' a b HA HB Ha Hb|]; [|constructor; tea].
+  assert (Hrw : forall A t, t[tRel 0 .: @wk1 Γ A >> tRel] = t).
+  { intros; bsimpl; apply idSubst_term; intros []; reflexivity. }
+  assert (Hrw' : forall a t, t[a .: @wk_id Γ >> tRel] = t[a..]).
+  { intros; now bsimpl. }
+  assert [Γ |-[ ta ] A].
+  { now unshelve eapply escape. }
+  assert [Γ |-[ ta ] A'].
+  { rewrite <- (wk_id_ren_on Γ A'); now unshelve eapply escapeConv, HA. }
+  assert [|-[ ta ] Γ,, A'].
+  { now eapply wfc_cons. }
+  assert [Γ |-[ ta ] A ≅ A'].
+  { rewrite <- (wk_id_ren_on Γ A), <- (wk_id_ren_on Γ A').
+    eapply escapeEq; now unshelve apply HA. }
+  assert (RB :
+    forall (Δ : context) (a : term) (ρ : Δ ≤ Γ) (h : [ |-[ ta ] Δ])
+       (ha : [PolyRedPack.shpRed (normRedΣ0 ΣA) ρ h | Δ ||- a
+             : (ParamRedTyPack.dom (normRedΣ0 ΣA))⟨ρ⟩]),
+     [Δ ||-<l> B[a .: ρ >> tRel]]
+  ).
+  { intros Δ a0 ? ? ha0.
+    unshelve econstructor.
+    + eapply PolyRedPack.posRed, ha0.
+    + eapply PolyRedPack.posAd, PolyRed.toAd. }
+  constructor; tea.
+  - rewrite <- (Hrw A' B); unshelve eapply escape, RB; tea.
+    apply var0conv; cbn; [|tea].
+    rewrite <- (@wk1_ren_on Γ A' A'); apply convty_wk; [tea|now symmetry].
+  - rewrite <- (Hrw A' B'); unshelve eapply escapeConv, HB; tea.
+    apply var0conv; cbn; [|tea].
+    rewrite <- (@wk1_ren_on Γ A' A'); apply convty_wk; [tea|now symmetry].
+  - rewrite <- (Hrw A B'); unshelve eapply escapeConv, HB.
+    + apply wfc_cons; tea.
+    + apply var0; cbn; [now bsimpl|tea].
+  - rewrite <- (Hrw A B), <- (Hrw A B'); unshelve eapply escapeEq, HB.
+    + apply wfc_cons; tea.
+    + apply var0; cbn; [now bsimpl|tea].
+  - rewrite <- (Hrw A' B), <- (Hrw A' B'); unshelve eapply escapeEq, HB.
+    + apply wfc_cons; tea.
+    + apply var0conv; cbn; tea.
+      rewrite <- (@wk1_ren_on Γ A' A'); apply convty_wk; [tea|now symmetry].
+  - rewrite <- (wk_id_ren_on Γ A), <- (wk_id_ren_on Γ a).
+    now unshelve eapply escapeTerm, Ha.
+  - rewrite <- Hrw'.
+    unshelve eapply escape, RB; tea.
+    rewrite <- (wk_id_ren_on Γ a); now unshelve apply Ha.
+  - rewrite <- Hrw'; unshelve eapply escapeConv, HB; tea.
+    rewrite <- (wk_id_ren_on Γ a); now unshelve apply Ha.
+  - rewrite <- !Hrw'; unshelve eapply escapeEq, HB; tea.
+    rewrite <- (wk_id_ren_on Γ a); now unshelve apply Ha.
+  - rewrite <- Hrw', <- (wk_id_ren_on Γ b), <- (wk_id_ren_on Γ a).
+    now unshelve eapply escapeTerm, Hb.
   Qed.
 
   Lemma isLRPair_isPair {Γ A B l p} (ΣA : [Γ ||-Σ<l> tSig A B]) (Rp : [Γ ||-Σ p : _ | normRedΣ0 ΣA]) :
